% \documentclass[compacto,10pt]{aleph-notas}
\documentclass[compacto,10pt,comentarios]{aleph-notas}

% -- Paquetes adicionales
\usepackage{enumitem}
\usepackage{aleph-comandos}
\usepackage{parskip}
\usepackage{graphicx}
\usepackage{xfrac}
\usepackage{tikz}
\usepackage{etoolbox}
\usepackage[framemethod=tikz]{mdframed}
\DeclareFontFamily{U}{skulls}{}
\DeclareFontShape{U}{skulls}{m}{n}{ <-> skull }{}
\newcommand{\skull}{\text{\usefont{U}{skulls}{m}{n}\symbol{'101}}}
\def \ds{\displaystyle}
\def \dfx{\dfrac{d}{dx}}
\DeclareMathOperator{\arccot}{arccot}
\DeclareMathOperator{\arcsec}{arcsec}
\DeclareMathOperator{\arccsc}{arccsc}
\newcommand*\Heq{\ensuremath{\overset{\kern2pt LH}{=}}}

% -- Datos del libro
\institucion{Southwestern College}
\asignatura{MATH 251: Calculus II}
\tema{Partial Fractions}
\autor{Jesús Pérez Cuarenta}
% \fecha{Fall 2024}

%% --> Logos de las guias
\logouno[4.5cm]{../Images/swc_logo}
\definecolor{colordef}{cmyk}{0.81, 0.62, 0.00, 0.22}

%% -- Solucion para alumnos
% \AtBeginEnvironment{proof}{\color{white}}

%% 
% https://www.emathhelp.net/en/calculators/algebra-2/partial-fraction-decomposition-calculator/

\begin{document}

\encabezado

\section*{Partial Fractions}
\begin{mdframed}
    \center Learning Objectives \\
    \begin{itemize}
        \item Evaluate integrals using partial fraction decomposition.
    \end{itemize}
\end{mdframed}

Let us consider the problem of combining two fractions such as
$$
    \frac{3}{x - 3} - \frac{2}{x - 2} ~ .
$$
The idea is to find the lowest common denominator (LCD) and build each fraction to an equivalent one with the LCD as the denominator, i.e.,
\begin{align*}
    \frac{3}{x - 3} - \frac{2}{x - 2} 
    & = \frac{3}{(x - 3)} \cdot \frac{(x - 2)}{(x - 2)} -  \frac{2}{(x - 2)} \cdot \frac{(x - 3)}{(x - 3)} \\
    & = \frac{x}{x^{2} -5x + 6} ~ .
\end{align*}

It is natural to ask if there is a procedure for taking the steps in reverse. Namely, how can we find constants $A$ and $B$ such that the following holds
\begin{align*}
    \frac{x}{x^{2} -5x + 6}
    & = \frac{A}{x - 3} + \frac{B}{x - 2} ~ .
\end{align*}

Let $f(x) = \frac{p(x)}{q(x)}$ be a rational polynomial function where $q(x) \neq 0$. We consider three cases
\begin{itemize}
    \item Case $q(x)$ has only nonrepeated linear factors \\
    Here, $q(x)$ is of the form
    $$
        q(x) = (x - a_1) (x - a_2) \ldots (x - a_n)
    $$
    where $i \neq j$ implies $a_i \neq a_j$. The decomposition is of the form
    $$
        \frac{p(x)}{q(x)} = \frac{A_1}{x-a_1} + \frac{A_2}{x - a_2} + \ldots + \frac{A_n}{x-a_n}
    $$
    where all the $A_i$ are to be determined.

    \item Case $q(x)$ has only repeated linear factors \\
    Here, $q(x)$ is of the form
    $$
        q(x) = (x - a) (x - a) \ldots (x - a) = (x - a)^{n}
    $$
    where $n \geq 2$. The decomposition is of the form
    $$
        \frac{p(x)}{q(x)} = \frac{A_1}{(x-a)} + \frac{A_2}{(x - a)^2} + \ldots + \frac{A_n}{(x-a)^n}
    $$
    where all the $A_i$ are to be determined.

    \item Case $q(x)$ has a nonrepeated irreducible quadratic factor \\
    Here, $q(x)$ is of the form
    $$
    ax^{2} + bx + c
    $$ 
    and the decomposition allows for the term
    $$
        \frac{Ax+B}{ax^{2} + bx + c}
    $$
    where $A$ and $B$ are to be determined.
\end{itemize}

\begin{ejer}
    Decompose
    $$
        f(x) = \frac{x}{x^{2} - 5x + 6}.
    $$
\end{ejer}
\begin{proof}[Solution]
    Notice that $f(x) = \frac{p(x)}{q(x)}$ is a rational polynomial function where
    $$
        q(x) = x^{2} - 5x + 6 = (x-3)(x+2)
    $$
    implies that $q(x)$ only has nonrepeated linear factors. Hence, we have
    \begin{align*}
        \frac{x}{x^{2} - 5x + 6}
        & = \frac{x}{(x - 3)(x - 2)} \\ 
        & = \frac{A}{(x - 3)} + \frac{B}{(x - 2)} \\
        & = \frac{\left(x - 3\right) B + \left(x - 2\right) A}{\left(x - 3\right) \left(x - 2\right)} ~ .
    \end{align*}
    Now we compare numerators,
    \begin{align*}
        x & = \left(x - 3\right) B + \left(x - 2\right) A \\
        & = x A + x B - 2 A - 3 B \\
        & = x \left(A + B\right) - 2 A - 3 B ~
    \end{align*}
    which is equivalent to solving the system of equations
    $$
        \begin{cases} A + B = 1\\-2 A - 3 B = 0 \end{cases}
    $$
    so that
    $$
        A = 3
    $$
    and
    $$
        B = -2 ~ .
    $$
    Finally,
    $$
        \frac{x}{\left(x - 3\right) \left(x - 2\right)}=\frac{3}{x - 3} - \frac{2}{x - 2} ~ .
    $$
\end{proof}

\begin{ejer}
    Integrate
    $$
        \int \frac{x}{x^{2} - 5x + 6} ~ dx ~ .
    $$
\end{ejer}
\begin{proof}[Solution]
    From the previous exercise, we have
    \begin{align*}
      \int \frac{x}{\left(x - 3\right) \left(x - 2\right)} ~ dx 
      & = \int \frac{3}{x - 3} - \frac{2}{x - 2} ~ dx \\
      & = 3\ln(|x - 3|) - 2 \ln(|x - 2|) + C ~ .
    \end{align*}
\end{proof}

In general, we will follow the steps.
\begin{itemize}
    \item Check if fraction is improper, if so apply long division.
    \item Factor the denominator.
    \item Write out the partial fraction decomposition.
\end{itemize}

\begin{ejer}
    Integrate
    $$
        \int \frac{2x-1}{4x^2 - 9} ~ dx.
    $$
\end{ejer}
\begin{proof}[Solution]
    Factor the denominator
    $$
        \frac{2 x - 1}{4 x^{2} - 9}=\frac{2 x - 1}{\left(2 x - 3\right) \left(2 x + 3\right)} ~ .
    $$
    The form of the partial fraction decomposition is
    $$
        \frac{2 x - 1}{\left(2 x - 3\right) \left(2 x + 3\right)}=\frac{A}{2 x - 3}+\frac{B}{2 x + 3} ~ .
    $$
    Write the right-hand side as a single fraction:
    $$
        \frac{2 x - 1}{\left(2 x - 3\right) \left(2 x + 3\right)}=\frac{\left(2 x - 3\right) B + \left(2 x + 3\right) A}{\left(2 x - 3\right) \left(2 x + 3\right)} ~ .
    $$
    The denominators are equal, so we require the equality of the numerators:
    $$
        2 x - 1=\left(2 x - 3\right) B + \left(2 x + 3\right) A ~ .
    $$
    Expand the right-hand side:
    $$
        2 x - 1=2 x A + 2 x B + 3 A - 3 B ~ .
    $$
    Collect like terms:
    $$
        2 x - 1=x \left(2 A + 2 B\right) + 3 A - 3 B ~ .
    $$
    The coefficients near the like terms should be equal, so the following system is obtained:
    $$
        \begin{cases} 2 A + 2 B = 2\\3 A - 3 B = -1 \end{cases}
    $$
    so that 
    $$
        A = \frac{1}{3}
    $$
    and
    $$
        B = \frac{2}{3} ~ .
    $$
    Hence,
    $$
        \frac{2 x - 1}{\left(2 x - 3\right) \left(2 x + 3\right)}=\frac{1}{3(2 x - 3)}+\frac{2}{3(2 x + 3)} ~ .
    $$
    Now we integrate,
    \begin{align*}
        \int \frac{2x-1}{4x^2 - 9} ~ dx
        & = \int \frac{2 x - 1}{\left(2 x - 3\right) \left(2 x + 3\right)} ~ dx \\ 
        & = \int \frac{1}{3(2 x - 3)} + \frac{2}{3(2 x + 3)} ~ dx \\
        & = \frac{1}{6} \ln(|2x-3|) + \frac{1}{3} \ln(|2x + 3|) + C .
    \end{align*}
\end{proof}

\begin{ejer}
    Integrate
    $$
        \int \frac{4x+7}{(x+1)^2} ~ dx.
    $$
\end{ejer}
\begin{proof}[Solution]
    The form of the partial fraction decomposition is
    $$
        \frac{4 x + 7}{\left(x + 1\right)^{2}}=\frac{A}{x + 1}+\frac{B}{\left(x + 1\right)^{2}} ~ .
    $$
    Write the right-hand side as a single fraction:
    $$
        \frac{4 x + 7}{\left(x + 1\right)^{2}}=\frac{\left(x + 1\right) A + B}{\left(x + 1\right)^{2}} ~ .
    $$
    The denominators are equal, so we require the equality of the numerators:
    $$
        4 x + 7=\left(x + 1\right) A + B ~ .
    $$
    Expand the right-hand side:
    $$
    4 x + 7=x A + A + B ~ .
    $$
    Collect like terms:
    $$
        4 x + 7=x A + A + B ~ .
    $$
    The coefficients near the like terms should be equal, so the following system is obtained:
    $$
        \begin{cases} A = 4\\A + B = 7 \end{cases} 
    $$
    so that 
    $$
        A = 4
    $$
    and
    $$
        B = 3 ~ .
    $$
    Hence,
    $$
        \frac{4 x + 7}{\left(x + 1\right)^{2}}=\frac{4}{x + 1}+\frac{3}{\left(x + 1\right)^{2}} ~ .
    $$
    Now we integrate,
    \begin{align*}
        \int \frac{4x+7}{(x+1)^2} ~ dx
        & = \int \frac{4}{x + 1}+\frac{3}{\left(x + 1\right)^{2}} ~ dx \\ 
        & = 4\ln(|x+1|) - \frac{3}{x+1} + C.
    \end{align*}
\end{proof}

\begin{ejer}
    Integrate
    $$
        \int \frac{2x+3}{x^3-2x^2+3x-6} ~ dx.
    $$
\end{ejer}
\begin{proof}
    Simplify the expression
    $$
        \frac{2 x + 3}{x^{3} - 2 x^{2} + 3 x - 6}=\frac{2 x + 3}{\left(x - 2\right) \left(x^{2} + 3\right)} ~ .
    $$
    The form of the partial fraction decomposition is
    $$
        \frac{2 x + 3}{\left(x - 2\right) \left(x^{2} + 3\right)}=\frac{A}{x - 2}+\frac{B x + C}{x^{2} + 3} ~ .
    $$
    Write the right-hand side as a single fraction:
    $$
        \frac{2 x + 3}{\left(x - 2\right) \left(x^{2} + 3\right)}=\frac{\left(x - 2\right) \left(B x + C\right) + \left(x^{2} + 3\right) A}{\left(x - 2\right) \left(x^{2} + 3\right)} ~ .
    $$
    The denominators are equal, so we require the equality of the numerators:
    $$
        2 x + 3=\left(x - 2\right) \left(B x + C\right) + \left(x^{2} + 3\right) A ~ .
    $$
    Expand the right-hand side:
    $$
        2 x + 3=x^{2} A + x^{2} B - 2 x B + x C + 3 A - 2 C ~ .
    $$
    Collect like terms:
    $$
        2 x + 3=x^{2} \left(A + B\right) + x \left(- 2 B + C\right) + 3 A - 2 C ~ .
    $$
    The coefficients near the like terms should be equal, so the following system is obtained:
    $$
        \begin{cases} A + B = 0\\- 2 B + C = 2\\3 A - 2 C = 3 \end{cases}
    $$
    so that
    $$
        A = 1, B = -1, \text{ and } C = 0 ~ .
    $$
    Hence,
    $$
        \frac{2 x + 3}{\left(x - 2\right) \left(x^{2} + 3\right)}=\frac{1}{x - 2} - \frac{x}{x^{2} + 3} ~ .
    $$
    Now we integrate,
    \begin{align*}
        \int \frac{2x+3}{x^3-2x^2+3x-6} ~ dx
        & = \int \frac{1}{x - 2}-\frac{x}{x^{2} + 3} ~ dx \\
        & = \ln(|x - 2|) - \frac{1}{2} \ln(x^2 + 3) + C ~ .
    \end{align*}

\end{proof}

\begin{ejer}
    Integrate
    $$
        \int \frac{x^3+x-3}{x^2 - 4} ~ dx.
    $$
\end{ejer}
\begin{proof}
    Since the fraction is improper, we use long division to get the following result
    $$
        \frac{x^{3} + x - 3}{x^{2} - 4}=x+\frac{5 x - 3}{x^{2} - 4} ~ .
    $$
    Now, we deal with the fractional part. Namely,
    $$
        \frac{5 x - 3}{x^{2} - 4} ~ .
    $$
    Factor the denominator:
    $$
        \frac{5 x - 3}{x^{2} - 4}=\frac{5 x - 3}{\left(x - 2\right) \left(x + 2\right)} ~ .
    $$
    The form of the partial fraction decomposition is
    $$
        \frac{5 x - 3}{\left(x - 2\right) \left(x + 2\right)}=\frac{A}{x - 2}+\frac{B}{x + 2} ~ .
    $$
    Write the right-hand side as a single fraction:
    $$
        \frac{5 x - 3}{\left(x - 2\right) \left(x + 2\right)}=\frac{\left(x - 2\right) B + \left(x + 2\right) A}{\left(x - 2\right) \left(x + 2\right)} ~ .
    $$
    The denominators are equal, so we require the equality of the numerators:
    $$
        5 x - 3=\left(x - 2\right) B + \left(x + 2\right) A ~ .
    $$
    Expand the right-hand side:
    $$
        5 x - 3=x A + x B + 2 A - 2 B ~ .
    $$
    Collect like terms:
    $$
        5 x - 3=x \left(A + B\right) + 2 A - 2 B ~ .
    $$
    The coefficients near the like terms should be equal, so the following system is obtained:
    $$
        \begin{cases} A + B = 5\\2 A - 2 B = -3 \end{cases}
    $$
    so that
    $$
    A = \frac{7}{4}
    $$
    and
    $$
    B = \frac{13}{4} ~ .
    $$
    Hence,
    $$
        \frac{5 x - 3}{\left(x - 2\right) \left(x + 2\right)}=\frac{7}{4(x - 2)}+\frac{13}{4(x + 2)} ~ .
    $$
    Now integrate,
    \begin{align*}
        \int \frac{x^3+x-3}{x^2 - 4} ~ dx
        & = \int x + \frac{7}{4(x - 2)}+\frac{13}{4(x + 2)} dx \\
        & = \frac{1}{4} \left( 2x^{2} + 7 \ln(|x-2|) + 13 \ln(x + 2) \right) + C ~ .
    \end{align*}
\end{proof}

\end{document}